src/lib/spec/Kuiper.Spec.Softmax.fsti
@@ -1,0 +1,12 @@
+module Kuiper.Spec.Softmax
+
+#lang-pulse
+open Kuiper
+open Kuiper.Array1
+open Kuiper.Seq.Common
+
+(* Real-value golden specification for softmax. *)
+let softmax_real (s:Seq.seq real { Seq.length s > 0 }) =
+  let exps = seq_map rexp s in
+  let summ : real = rsum exps in
+  seq_map (fun x -> rexp x /. summ) s
